Big and small step inductively defined

Smallstep.v
@@ -1,4 +1,88 @@
 Require Export Imp.
 
+Inductive tm: Type :=
+| C : nat -> tm         (* Constant *)
+| P : tm -> tm -> tm.   (* Plus *)
+
+Tactic Notation "tm_cases" tactic(first) ident(c) :=
+    first;
+    [ Case_aux c "C" | Case_aux c "P" ].
+
+(* big-step style *)
+
+Fixpoint evalF (t : tm) : nat :=
+    match t with
+    | C n => n
+    | P a1 a2 => evalF a1 + evalF a2
+    end.
+
+Reserved Notation " t '|| n " (at level 50, left associativity).
+
+Inductive eval : tm -> nat -> Prop :=
+| E_Const : forall n,
+        C n || n
+| E_Plus : forall t1 t2 n1 n2,
+        t1 || n1 ->
+        t2 || n2 ->
+        P t1 t2 || (n1 + n2)
+
+where " t '||' n " := (eval t n).
+
+Tactic Notation "eval_cases" tactic(first) ident(c) :=
+    first;
+    [ Case_aux c "E_Const" | Case_aux c "E_Plus" ].
+
+Module SimpleArith1.
+
+Reserved Notation " t '==>' t' " (at level 40).
+
+Inductive step : tm -> tm -> Prop :=
+  (* the only reduction step *)
+| ST_PlusConstConst : forall n1 n2,
+        P (C n1) (C n2) ==> C (n1 + n2)
+  (* expand on t1, eventually reaching state
+     where the first or third rule apply *)
+| ST_Plus1 : forall t1 t1' t2,
+        t1 ==> t1' ->
+        P t1 t2 ==> P t1' t2
+  (* t1 now must be a constant, expand on t2,
+     eventually reaching state where
+     the first or second rule apply *)
+| ST_Plus2: forall n1 t2 t2',
+        t2 ==> t2' ->
+        P (C n1) t2 ==> P (C n1) t2'
+
+where " t '==>' t' " := (step t t').
+
+Tactic Notation "step_cases" tactic(first) ident(c) :=
+    first;
+    [ Case_aux c "ST_PlusConstConts"
+    | Case_aux c "ST_Plus1" | Case_aux c "ST_Plus2" ].
+
+Example test_step_1 :
+    P (P (C 0) (C 3))
+      (P (C 2) (C 4))
+    ==>
+    P (C (0 + 3))
+      (P (C 2) (C 4)).
+Proof.
+    apply ST_Plus1. apply ST_PlusConstConst.
+Qed.
+
+Example test_step_2 :
+    P (C 0)
+      (P (C 2)
+         (P (C 0) (C 3)))
+    ==>
+    P (C 0)
+      (P (C 2)
+         (C (0 + 3))).
+Proof.
+    apply ST_Plus2. apply ST_Plus2. apply ST_PlusConstConst.
+Qed.
+
+
+
+
 
 
